\documentclass[../SOP.tex]{subfile}

\begin{document}
\begin{gather}
  E_t(\mathbf{o})=\frac{1}{2}\sum_{k=1}^n(t_k-o_k)^2 \label{eq:cost}\\
  E_t\colon \R^n\rightarrow\R\nonumber
\end{gather}
\begin{equation}
  E(\mathbf{w})=\frac{1}{2}\sum_{t\in T}\sum_{k\in outputs}(t_{kd}-o_{kd})^2
  \label{eq:costset}
\end{equation}
\begin{equation*}
  P=\frac{c}{t}
\end{equation*}
\begin{equation}
  \nabla E(\mathbf{w})=\begin{bmatrix}
    \pfrac{E}{w_0} & \pfrac{E}{w_1} & \dots & \pfrac{E}{w_n}
  \end{bmatrix}
  \label{eq:gradError}
\end{equation}
\begin{gather}
  \Delta \mathbf{w} = -\eta \nabla E(\mathbf{w}) \label{eq:trgrad}\\ 
  \mathbf{w} \leftarrow \mathbf{w} + \Delta\mathbf{w}
\end{gather}
\begin{equation*}
  E(w_{jk})=\frac{1}{2}(t_j-\sigma(w_{jk}o_k))^2
\end{equation*}
\begin{equation*}
  \pfrac{E}{w_{jk}}=\pfrac{E}{o_j}\cdot\pfrac{o_j}{x_j}\cdot\pfrac{x_j}{w_{jk}}
\end{equation*}
\begin{equation*}
  \pfrac{x_j}{w_{jk}}=o_k
\end{equation*}
\begin{align*}
  \pfrac{E}{o_j}&=\pfrac{}{o_j}\frac{1}{2}(t_j-o_j)^2\\
  &= (t_j-o_j)\pfrac{}{o_j}(t_j-o_j)\\
  &= (t_j-o_j)\cdot-1\\
  &= -(t_j-o_j)
\end{align*}
\begin{equation*}
  \sigma'(x)=\sigma(x)\cdot(1-\sigma(x))
\end{equation*}
\begin{equation*}
  \pfrac{o_j}{x_j}=\pfrac{\sigma(x_j)}{x_j}=o_j\cdot(1-o_j)
\end{equation*}
\begin{equation}
  \pfrac{E}{w_jk}=(t_j-o_j)\cdot o_j \cdot (1-o_j)\cdot o_k
  \label{eq:errorWeight}
\end{equation}
\begin{equation}
  \Delta w_{jk}=\eta\cdot (t_j-o_j)\cdot o_j\cdot(1-o_j)\cdot o_k
  \label{eq:trOutput}
\end{equation}
\begin{equation}
  \delta_j =-\pfrac{E}{x_j}=o_j\cdot(1-o_j)\cdot(t_j-o_j)
  \label{eq:delta}
\end{equation}
\begin{equation*}
  \pfrac{x_j}{w_{jk}}=o_k
\end{equation*}
\begin{align*}
  \pfrac{E}{x_j}&=\sum_{k\in Ds(j)} \pfrac{E}{x_k}\cdot \pfrac{x_k}{x_j}\\
  \intertext{$\delta_k$ kan nu indf√∏res, jf. ligning \ref{eq:delta}}
  \pfrac{E}{x_j}&=\sum_{k\in Ds(j)} -\delta_k\cdot \pfrac{x_k}{x_j}\\
  &= \sum_{k\in Ds(j)} -\delta_k \cdot \pfrac{x_k}{o_j}\cdot\pfrac{o_j}{x_j}\\
  &= \sum_{k\in Ds(j)} -\delta_k \cdot w_{kj}\cdot \pfrac{o_j}{x_j}\\
  &= \sum_{k\in Ds(j)} -\delta_k \cdot w_{kj}\cdot o_j\cdot(1-o_j)\\
  &= o_j\cdot(1-o_j)\sum_{k\in Ds(j)} -\delta_k \cdot w_{kj}
\end{align*}
\begin{equation}
  \delta_j=o_j\cdot(1-o_j)\cdot\sum_{k\in Ds(j)} \delta_k\cdot w_{kj} 
  \label{eq:delta_h}
\end{equation}
\begin{equation}
  \Delta w_{jk}=\eta\cdot \delta_j\cdot o_{k}
  \label{eq:wchange}
\end{equation}
      \begin{equation*}
        \delta_k = o_k\cdot (1-o_k)\cdot(t_k-o_k)
      \end{equation*}
      \begin{equation*}
        \delta_h = o_h\cdot(1-o_h) \sum_{k\in Ds(h)} w_{kh}\delta_k
      \end{equation*}
      \begin{equation*}
        \Delta w_{jk} = \eta\cdot\delta_j\cdot o_k
      \end{equation*}
      \begin{equation*}
        w_{jk} \leftarrow \Delta w_{jk} + w_{jk}
      \end{equation*}
      \end{document}
