\documentclass[../SOP.tex]{subfile}

\begin{document}
\begin{equation*}
  \bm{v} = \begin{bmatrix} 1 \\ 2 \\ 3 \\ 4 \end{bmatrix} \in \R^4
\end{equation*}
\begin{equation*}
  \begin{bmatrix}
    a_1 \\ b_1 \\ c_1 \\ \vdots
  \end{bmatrix}
  +
  \begin{bmatrix}
   a_2 \\ b_2 \\ c_2 \\ \vdots
  \end{bmatrix}
  =
  \begin{bmatrix}
    a_1+a_2 \\ b_1+b_2 \\ c_1+c_2 \\ \vdots
  \end{bmatrix}
\end{equation*}
\begin{equation*}
  \lambda 
  \begin{bmatrix}
    a \\ b \\ c \\ \vdots
  \end{bmatrix}
  =
  \begin{bmatrix}
    \lambda a \\ \lambda b \\ \lambda c \\ \vdots
  \end{bmatrix}
\end{equation*}
\begin{equation*}
  \begin{bmatrix}
    a_1 \\ b_1 \\ c_1 \\ \vdots
  \end{bmatrix}
  \cdot
  \begin{bmatrix}
    a_2 \\ b_2 \\ c_2 \\ \vdots
  \end{bmatrix}
  = a_1a_2 + b_1b_2 + c_1c_2
\end{equation*}
\begin{gather*}
  a=\begin{bmatrix}
    a_1 \\ a_2 \\ \vdots
  \end{bmatrix}
  \\
  a^T=\begin{bmatrix}
    a_1 & a_2 & \cdots
  \end{bmatrix}
\end{gather*}
\begin{equation*}
  \begin{bmatrix}
    a_1 \\ b_1 \\ c_1
  \end{bmatrix}
  \otimes
  \begin{bmatrix}
    a_2 \\ b_2 \\ c_2
  \end{bmatrix}
  =
  \begin{bmatrix}
  a_1a_2 & a_1b_2 & a_1c_2 \\
  b_1a_2 & b_1b_2 & b_1c_2 \\
  c_1a_2 & c_1b_2 & c_1c_2
  \end{bmatrix}
\end{equation*}
\begin{equation*}
  \mathbf{A}=\begin{bmatrix}
    a_{11} & a_{12} & \cdots & a_{1n} \\
    a_{21} & a_{22} & \cdots & a_{2n} \\
    \vdots & \vdots & \ddots & \vdots \\
    a_{m1} & a_{m2} & \cdots & a_{mn}
  \end{bmatrix}
  \in \R^{m\times n}
\end{equation*}
\begin{equation*}
  \begin{bmatrix}
    a_{11} & a_{12} & \cdots & a_{1n} \\
    a_{21} & a_{22} & \cdots & a_{2n} \\
    \vdots & \vdots & \ddots & \vdots \\
    a_{m1} & a_{m2} & \cdots & a_{mn}
  \end{bmatrix}
  +
  \begin{bmatrix}
    b_{11} & b_{12} & \cdots & b_{1n} \\
    b_{21} & b_{22} & \cdots & b_{2n} \\
    \vdots & \vdots & \ddots & \vdots \\
    b_{m1} & b_{m2} & \cdots & b_{mn}
  \end{bmatrix}
  =
  \begin{bmatrix}
    a_{11} + b_{11} & a_{12} + b_{12} & \cdots \\
    a_{21} + b_{21} & a_{22} + b_{22} & \cdots \\
    \vdots & \vdots & \ddots \\
    a_{m1} + b_{m1} & a_{m2} + b_{m2} & \cdots 
  \end{bmatrix}
\end{equation*}
\begin{equation*}
  \lambda
  \begin{bmatrix}
    a_{11} & a_{12} & \cdots & a_{1n} \\
    a_{21} & a_{22} & \cdots & a_{2n} \\
    \vdots & \vdots & \ddots & \vdots \\
    a_{m1} & a_{m2} & \cdots & a_{mn}
  \end{bmatrix}
  =
  \begin{bmatrix}
    \lambda a_{11} & \lambda a_{12} & \cdots & \lambda a_{1n} \\
    \lambda a_{21} & \lambda a_{22} & \cdots & \lambda a_{2n} \\
    \vdots & \vdots & \ddots & \vdots \\
    \lambda a_{m1} & \lambda a_{m2} & \cdots & \lambda a_{mn}
  \end{bmatrix}
\end{equation*}
\begin{align*}
  c_{ij} &= \sum_{l=1}^n a_{il}b_{lj}\\
  i&=1,\dots,m\\
  j&=1,\dots,k
\end{align*}
\begin{equation*}
  \mathbf{A}\cdot\mathbf{B}\neq\mathbf{B}\cdot\mathbf{A}
\end{equation*}
\begin{gather*}
  \underbrace{\mathbf{A}}_{n\times k}\cdot\underbrace{\mathbf{B}}_{k\times m}=\underbrace{\mathbf{C}}_{n\times m}\\
  k=k\\
  \underbrace{\mathbf{B}}_{k\times m}\cdot\underbrace{\mathbf{A}}_{n\times k}=\ ?\\
  m\neq n
\end{gather*}
\begin{equation*}
  \begin{bmatrix}
    a_{11} & a_{12} \\
    a_{21} & a_{22} \\
    a_{31} & a_{32}
  \end{bmatrix}
  \cdot
  \begin{bmatrix}
    b_1 \\ b_2
  \end{bmatrix}
  =
  \begin{bmatrix}
    a_{11}b_1 + a_{12}b_2\\
    a_{21}b_1 + a_{22}b_2 \\
    a_{31}b_1 + a_{32}b_2
  \end{bmatrix}
\end{equation*}
\begin{gather*}
  A_{ij}=(A^T)_{ji}\\
  A\in \R^{n\times m}\\
  A^T \in \R^{m\times n}
\end{gather*}
\begin{equation*}
  \begin{bmatrix}
  a_1 \\ b_1 \\ c_1
  \end{bmatrix}
  \odot
  \begin{bmatrix}
    a_2 \\ b_2 \\ c_2
  \end{bmatrix}
  =
  \begin{bmatrix}
    a_1a_2 \\ b_1b_2 \\ c_1c_2
  \end{bmatrix}
\end{equation*}
\begin{equation*}
  f\colon Dm \rightarrow Vm
\end{equation*}
\begin{equation*}
  f\colon \R^3 \rightarrow \R
\end{equation*}
\begin{gather*}
  f(x,y)=xy^2+2+x^2\\
  \pfrac{f}{x}=y^2+2x\\
  \pfrac{f}{y}=2xy
\end{gather*}
\begin{equation*}
  \nabla f(x,y) = \begin{bmatrix}
    \pfrac{f}{x} & \pfrac{f}{y}
  \end{bmatrix}
  =
  \begin{bmatrix}
    y^2+2x & 2xy
  \end{bmatrix}
\end{equation*}
\end{document}
